generalize Hash and Timestamp types

Structures/Blocks.v
@@ -11,22 +11,20 @@ Set Implicit Arguments.
 Unset Strict Implicit.
 Unset Printing Implicit Defensive.
 
-Definition Hash := [ordType of nat].
-
-Record Block {Transaction VProof : eqType} :=
+Record Block {Hash : ordType} {Transaction VProof : eqType} :=
   mkB {
     prevBlockHash : Hash;
     txs : seq Transaction;
     proof : VProof;
   }.
 
-Definition eq_block {T P : eqType} (b b' : @Block T P) :=
+Definition eq_block {H : ordType} {T P : eqType} (b b' : @Block H T P) :=
   match (b, b') with
   | (mkB p t pf, mkB p' t' pf') =>
     [&& p == p', t == t' & pf == pf']
   end.
       
-Lemma eq_blockP {T P : eqType} : Equality.axiom (@eq_block T P).
+Lemma eq_blockP {H : ordType} {T P : eqType} : Equality.axiom (@eq_block H T P).
 Proof.
 case=> p t pf; case=> p' t' pf'; rewrite /eq_block/=.
 case H2: (p == p'); [move/eqP: H2=>?; subst p'| constructor 2];
@@ -38,8 +36,8 @@ case H4: (pf == pf'); [move/eqP: H4=>?; subst pf'| constructor 2];
 by constructor 1. 
 Qed.
 
-Canonical Block_eqMixin {T P : eqType} :=
-  Eval hnf in EqMixin (@eq_blockP T P).
-Canonical Block_eqType {T P : eqType} :=
-  Eval hnf in EqType (@Block T P) (@Block_eqMixin T P).
+Canonical Block_eqMixin {H : ordType} {T P : eqType} :=
+  Eval hnf in EqMixin (@eq_blockP H T P).
+Canonical Block_eqType {H : ordType} {T P : eqType} :=
+  Eval hnf in EqType (@Block H T P) (@Block_eqMixin H T P).
 
